src/typechecker/FStar.TypeChecker.Env.fs
@@ -68,6 +68,8 @@ type step =
   | Unascribe
   | NBE
   | ForExtraction //marking an invocation of the normalizer for extraction
+  | OnExtractionOnly // only used for norm requests, to mark that they should be
+                     // only interpreted at extraction time
 and steps = list<step>
 
 let rec eq_step s1 s2 =
