ulib/FStar.Pervasives.fsti
@@ -772,6 +772,8 @@ val primops : norm_step
 (** Unfold all non-recursive definitions *)
 val delta : norm_step
 
+val on_extraction_only : norm_step
+
 (** Unroll recursive calls
 
     Note: Since F*'s termination check is semantic rather than
